Section 3.1

analysis/Analysis/Section_3_1.lean
@@ -80,19 +80,35 @@ class SetTheory where
   set_to_object : Set ↪ Object -- Axiom 3.1
   mem : Object → Set → Prop -- Axiom 3.1
   extensionality X Y : (∀ x, mem x X ↔ mem x Y) → X = Y -- Axiom 3.2
+
+  univ : Set
+  mem_univ x : mem x univ
+
   emptyset: Set -- Axiom 3.3
   emptyset_mem x : ¬ mem x emptyset -- Axiom 3.3
+
   singleton : Object → Set -- Axiom 3.4
   singleton_axiom x y : mem x (singleton y) ↔ x = y -- Axiom 3.4
   union_pair : Set → Set → Set -- Axiom 3.5
   union_pair_axiom X Y x : mem x (union_pair X Y) ↔ (mem x X ∨ mem x Y) -- Axiom 3.5
-  specify A (P: Subtype (mem . A) → Prop) : Set -- Axiom 3.6
-  specification_axiom A (P: Subtype (mem . A) → Prop) :
+
+  specify A (P: Subtype (mem · A) → Prop) : Set -- Axiom 3.6
+
+  specification_axiom A (P: Subtype (mem · A) → Prop) :
     (∀ x, mem x (specify A P) → mem x A) ∧ ∀ x, mem x.val (specify A P) ↔ P x -- Axiom 3.6
-  replace A (P: Subtype (mem . A) → Object → Prop)
-    (hP: ∀ x y y', P x y ∧ P x y' → y = y') : Set -- Axiom 3.7
-  replacement_axiom A (P: Subtype (mem . A) → Object → Prop)
-    (hP: ∀ x y y', P x y ∧ P x y' → y = y') : ∀ y, mem y (replace A P hP) ↔ ∃ x, P x y -- Axiom 3.7
+
+  -- Axiom 3.7
+  replace A -- “Let A be a set”
+    (P: Subtype (mem · A) → Object → Prop) -- “a statement P(x, y) pertaining to x ∈ A and any object y”
+    (hP: ∀ x y y', P x y ∧ P x y' → y = y') -- “there is at most one y for which P(x, y) is true”
+    : Set -- “then there exists a set {y : P(x, y) is true for some x}”
+
+  -- Axiom 3.7
+  replacement_axiom A -- “Let A be a set”
+    (P : Subtype (mem · A) → Object → Prop) -- “a statement P(x, y) pertaining to x ∈ A and any object y”
+    (hP : ∀ x y y', P x y ∧ P x y' → y = y') -- “there is at most one y for which P(x, y) is true”
+    : ∀ z, mem z (replace A P hP) ↔ ∃ x, P x z -- “then for any object z, z ∈ {y : ∃x, P(x, y)} iff ∃x ∈ A, P(x, z) is true”
+
   nat : Set -- Axiom 3.8
   nat_equiv : ℕ ≃ Subtype (mem . nat) -- Axiom 3.8
   regularity_axiom A (hA : ∃ x, mem x A) :
@@ -159,6 +175,9 @@ open SetTheory.Set
 @[simp]
 theorem SetTheory.Set.not_mem_empty : ∀ x, x ∉ (∅:Set) := emptyset_mem
 
+lemma SetTheory.Set.not_mem_empty' {x : Object} (h : x ∈ (∅:Set)) : False :=
+  ((not_mem_empty x) h).elim
+
 lemma SetTheory.Set.mem_empty_iff (x : Object) : x ∈ (∅:Set) ↔ False := by
   constructor
   . intro (h : x ∈ ∅)
@@ -167,26 +186,25 @@ lemma SetTheory.Set.mem_empty_iff (x : Object) : x ∈ (∅:Set) ↔ False := by
     exact h.elim
 
 /-- Empty set has no elements -/
-theorem SetTheory.Set.eq_empty_iff_forall_notMem {X : Set} :
+theorem SetTheory.Set.eq_empty_iff_forall_not_mem {X : Set} :
   X = ∅ ↔ (∀x, x ∉ X)
 := by
   constructor
   . -- ⊢ X = ∅ → ∀x, x ∉ X
     intro (hX : X = ∅) x
-    have h₁ : x ∉ ∅ := Set.not_mem_empty x
+    have h₁ : x ∉ ∅ := not_mem_empty x
     have h₂ : x ∉ X := hX ▸ h₁
     exact h₂
   . -- ⊢ (∀x, x ∉ X) → X = ∅
     intro (hX : ∀x, x ∉ X)
-    apply SetTheory.extensionality
-    intro y
+    ext y
     constructor
     . -- ⊢ y ∈ X → y ∈ ∅
       intro (hy : y ∈ X)
       exact ((hX y : y ∉ X) hy).elim
     . -- ⊢ y ∈ ∅ → y ∈ X
       intro (hy : y ∈ (∅:Set))
-      exact ((Set.not_mem_empty y : y ∉ ∅) hy).elim
+      exact ((not_mem_empty y : y ∉ ∅) hy).elim
 
 /-- Empty set is unique -/
 theorem SetTheory.Set.empty_unique : ∃! (X:Set), ∀ x, x ∉ X := by
@@ -195,20 +213,20 @@ theorem SetTheory.Set.empty_unique : ∃! (X:Set), ∀ x, x ∉ X := by
   -- ⊢ ∀ (Y:Set), (∀ (x:object), x ∉ Y) → Y = ∅
   intro X (hx : ∀x, x ∉ X)
   -- ⊢ X = ∅
-  exact (eq_empty_iff_forall_notMem.mpr : (∀x, x ∉ X) → X = ∅) hx
+  exact (eq_empty_iff_forall_not_mem.mpr : (∀x, x ∉ X) → X = ∅) hx
 
 /-- Lemma 3.1.5 (Single choice) -/
 lemma SetTheory.Set.nonempty_def {X:Set} (h: X ≠ ∅) : ∃ x, x ∈ X := by
   contrapose! h
   -- h: ∀x, x ∉ X
   -- ⊢ X = ∅
-  exact (eq_empty_iff_forall_notMem.mpr : (∀x, x ∉ X) → X = ∅) h
+  exact (eq_empty_iff_forall_not_mem.mpr : (∀x, x ∉ X) → X = ∅) h
 
 theorem SetTheory.Set.nonempty_of_inhabited {X:Set} {x:Object} (h:x ∈ X) : X ≠ ∅ := by
   contrapose! h
   -- h: X = ∅
   -- ⊢ x ∉ ∅
-  exact (eq_empty_iff_forall_notMem.mp : X = ∅ → ∀x, x ∉ X) h x
+  exact (eq_empty_iff_forall_not_mem.mp : X = ∅ → ∀x, x ∉ X) h x
 
 instance SetTheory.Set.instSingleton : Singleton Object Set where
   singleton := singleton
@@ -224,6 +242,12 @@ example (x: Object) : {x} = SetTheory.singleton x := rfl
 @[simp]
 theorem SetTheory.Set.mem_singleton (x a:Object) : x ∈ ({a}:Set) ↔ x = a := singleton_axiom x a
 
+lemma SetTheory.Set.mem_singleton' (x : Object) : x ∈ ({x} : Set) := (mem_singleton x x).mpr rfl
+
+lemma SetTheory.Set.eq_of_mem_singleton {x a : Object} (hxa : x ∈ ({a} : Set)) : x = a := (mem_singleton x a).mp hxa
+
+lemma SetTheory.Set.mem_singleton_of_eq {x a : Object} (hxa : x = a) : x ∈ ({a} : Set) := (mem_singleton x a).mpr hxa
+
 
 instance SetTheory.Set.instUnion : Union Set where
   union := union_pair
@@ -233,8 +257,23 @@ example (X Y: Set) : X ∪ Y = SetTheory.union_pair X Y := rfl
 
 /-- Axiom 3.4 (Pairwise union)-/
 @[simp]
-theorem SetTheory.Set.mem_union (x:Object) (X Y:Set) : x ∈ (X ∪ Y) ↔ (x ∈ X ∨ x ∈ Y) :=
+theorem SetTheory.Set.mem_union (x : Object) (X Y : Set) : x ∈ (X ∪ Y) ↔ (x ∈ X ∨ x ∈ Y) :=
   union_pair_axiom X Y x
+
+lemma SetTheory.Set.mem_union_left {x : Object} {X Y : Set}
+  (h : x ∈ X) : x ∈ X ∪ Y
+:= by
+  exact (mem_union x X Y).mpr (Or.inl h)
+
+lemma SetTheory.Set.mem_union_right {x : Object} {X Y : Set}
+  (h : x ∈ Y) : x ∈ X ∪ Y
+:= by
+  exact (mem_union x X Y).mpr (Or.inr h)
+
+lemma SetTheory.Set.mem_union_cases {x : Object} {X Y : Set}
+  (h : x ∈ X ∪ Y) : x ∈ X ∨ x ∈ Y
+:= by
+  exact (mem_union x X Y).mp h
 
 instance SetTheory.Set.instInsert : Insert Object Set where
   insert x X := {x} ∪ X
@@ -268,6 +307,13 @@ theorem SetTheory.Set.mem_pair (x a b:Object) : x ∈ ({a,b}:Set) ↔ (x = a ∨
       have hb₄ : x ∈ ({a, b}:Set)          := pair_eq a b ▸ hb₃
       exact hb₄
 
+lemma SetTheory.Set.mem_pair_left (x a b : Object) (h : x = a) : x ∈ ({a, b} : Set) :=
+  (mem_pair x a b).mpr (Or.inl h)
+
+lemma SetTheory.Set.mem_pair_right (x a b : Object) (h : x = b) : x ∈ ({a, b} : Set) :=
+  (mem_pair x a b).mpr (Or.inr h)
+
+
 @[simp]
 theorem SetTheory.Set.mem_triple (x a b c:Object) : x ∈ ({a,b,c}:Set) ↔ (x = a ∨ x = b ∨ x = c) := by
   constructor
@@ -289,7 +335,7 @@ theorem SetTheory.Set.singleton_uniq (a:Object) : ∃! (X:Set), ∀ x, x ∈ X �
   -- ⊢ ∀ X, (∀ x, x ∈ X ↔ x = a) → X = {a}
   intro X (h₀ : ∀ x, x ∈ X ↔ x = a)
   -- ⊢ X = {a}
-  apply SetTheory.extensionality
+  apply extensionality
   -- ⊢ ∀ x, x ∈ X ↔ x ∈ {a}
   intro x
   constructor
@@ -311,7 +357,7 @@ theorem SetTheory.Set.pair_uniq (a b:Object) : ∃! (X:Set), ∀ x, x ∈ X ↔ 
   -- ⊢ ∀ X, (∀ x, x ∈ X ↔ x = a ∨ x = b) → X = {a, b}
   intro X h₀
   -- ⊢ X = {a, b}
-  apply SetTheory.extensionality
+  apply extensionality
   -- ⊢ x ∈ X ↔ x ∈ {a, b}
   intro x
   have h₁ : x ∈ X ↔ x = a ∨ x = b              := h₀ x
@@ -321,8 +367,7 @@ theorem SetTheory.Set.pair_uniq (a b:Object) : ∃! (X:Set), ∀ x, x ∈ X ↔ 
 
 /-- Remark 3.1.9 -/
 theorem SetTheory.Set.pair_comm (a b:Object) : ({a,b}:Set) = {b,a} := by
-  apply SetTheory.extensionality
-  intro x
+  ext x
   constructor
   . intro (hxab : x ∈ ({a, b}:Set))
     have h₁ : x = a ∨ x = b    := (mem_pair x a b).mp hxab
@@ -336,8 +381,7 @@ theorem SetTheory.Set.pair_comm (a b:Object) : ({a,b}:Set) = {b,a} := by
 /-- Remark 3.1.9 -/
 @[simp]
 theorem SetTheory.Set.pair_self (a:Object) : ({a,a}:Set) = {a} := by
-  apply SetTheory.extensionality
-  intro x
+  ext x
   constructor
   . intro (hxaa : x ∈ ({a, a}:Set))
     have h₁ : x = a ∨ x = a := (mem_pair x a a).mp hxaa
@@ -446,24 +490,23 @@ theorem SetTheory.Set.union_congr_right (A B B':Set) (h: B = B') : A ∪ B = A �
 
 /-- Lemma 3.1.12 (Basic properties of unions) / Exercise 3.1.3 -/
 theorem SetTheory.Set.singleton_union_singleton (a b:Object) : ({a}:Set) ∪ ({b}:Set) = {a,b} := by
-  apply SetTheory.extensionality
-  exact fun x => ⟨
+  ext x
+  exact ⟨
     fun hx => (by simpa only [mem_union,  mem_singleton, ← mem_pair ] using hx),
     fun hx => (by simpa only [mem_pair, ← mem_singleton, ← mem_union] using hx),
   ⟩
 
 /-- Lemma 3.1.12 (Basic properties of unions) / Exercise 3.1.3 -/
 theorem SetTheory.Set.union_comm (A B:Set) : A ∪ B = B ∪ A := by
-  apply SetTheory.extensionality
-  exact fun x => ⟨
+  ext x
+  exact ⟨
     fun hx => (mem_union x B A).mpr ((mem_union x A B).mp hx).symm,
     fun hx => (mem_union x A B).mpr ((mem_union x B A).mp hx).symm,
   ⟩
 
 /-- Lemma 3.1.12 (Basic properties of unions) / Exercise 3.1.3 -/
 theorem SetTheory.Set.union_assoc (A B C:Set) : (A ∪ B) ∪ C = A ∪ (B ∪ C) := by
-  apply SetTheory.extensionality
-  intro x
+  ext x
   constructor
   . intro (h₀ : x ∈ A ∪ B ∪ C)
     have h₁ : (x ∈ A ∪ B) ∨ x ∈ C     := (mem_union x (A ∪ B) C).mp h₀
@@ -483,8 +526,7 @@ theorem SetTheory.Set.union_assoc (A B C:Set) : (A ∪ B) ∪ C = A ∪ (B ∪ C
 /-- Proposition 3.1.27(c) -/
 @[simp]
 theorem SetTheory.Set.union_self (A:Set) : A ∪ A = A := by
-  apply SetTheory.extensionality
-  intro x
+  ext x
   constructor
   . intro (h₀ : x ∈ A ∪ A)
     have h₁ : x ∈ A ∨ x ∈ A := (mem_union x A A).mp h₀
@@ -498,8 +540,7 @@ theorem SetTheory.Set.union_self (A:Set) : A ∪ A = A := by
 /-- Proposition 3.1.27(a) -/
 @[simp]
 theorem SetTheory.Set.union_empty (A:Set) : A ∪ ∅ = A := by
-  apply SetTheory.extensionality
-  intro x
+  ext x
   constructor
   . intro (h₀ : x ∈ A ∪ ∅)
     have h₁ : x ∈ A ∨ x ∈ (∅:Set) := (mem_union x A ∅).mp h₀
@@ -579,8 +620,7 @@ theorem SetTheory.Set.subset_trans {A B C:Set} (hAB:A ⊆ B) (hBC:B ⊆ C) : A �
 
 /-- Proposition 3.1.17 (Partial ordering by set inclusion) -/
 theorem SetTheory.Set.subset_antisymm (A B:Set) (hAB:A ⊆ B) (hBA:B ⊆ A) : A = B := by
-  apply SetTheory.extensionality
-  intro x
+  ext x
   have h₁ : x ∈ A → x ∈ B := hAB x
   have h₂ : x ∈ B → x ∈ A := hBA x
   have h₃ : x ∈ A ↔ x ∈ B := iff_def.mpr ⟨h₁, h₂⟩
@@ -678,7 +718,7 @@ theorem SetTheory.Set.ssubset_of_ssubset_of_subset' {A B C : Set} (hAB : A ⊂ B
   The object `x` associated to a subtype element `x'` is recovered as `x'.val`, and
   the property `hx` that `x` belongs to `A` is recovered as `x'.property`.
 -/
-abbrev SetTheory.Set.toSubtype (A:Set) := Subtype (fun x ↦ x ∈ A)
+abbrev SetTheory.Set.toSubtype (A:Set) := Subtype (· ∈ A)
 
 example (A: Set) (x: Object) (hx: x ∈ A) : A.toSubtype := ⟨x, hx⟩
 example (A: Set) (x': A.toSubtype) : Object := x'.val
@@ -692,6 +732,21 @@ example (A B: Set) (x': A.toSubtype) : x'.val ∈ A ∪ B := by simp; left; exac
 instance : CoeSort (Set) (Type v) where
   coe A := A.toSubtype
 
+structure Subtype' {α : Sort u} (p : α → Prop) where
+  val : α
+  property : p val
+abbrev SetTheory.Set.toSubtype' (A : Set) := Subtype' (· ∈ A)
+
+instance subtypeCoe' {α : Sort u} {p : α → Prop} : CoeOut (Subtype' p) α where
+  coe v := v.val
+
+example (A B : Set) (x : A.toSubtype') : x.val ∈ A ∪ B := by simp; left; exact x.property
+example (A : Set) (x : A.toSubtype') : x.val = x := by
+  have h := ↑x
+  rfl
+
+-- example (A : Set) (x : Object) (y : Object) (hx : x ∈ A) (hy : y ∈ A) :
+
 -- Now instead of writing `x': A.toSubtype`, we can just write `x': A`.
 -- Compare these three proofs. They are equivalent, but the last one reads most concisely.
 example (A B: Set) (x: Object) (hx: x ∈ A) : x ∈ A ∪ B := by simp; left; exact hx
@@ -704,7 +759,10 @@ example (A B: Set) (x': A) : x'.val ∈ A ∪ B := by simp; left; exact x'.prope
 -/
 lemma SetTheory.Set.subtype_property (A:Set) (x:A) : x.val ∈ A := x.property
 
-lemma SetTheory.Set.subtype_coe (A:Set) (x:A) : x.val = x := rfl
+lemma SetTheory.Set.subtype_coe (A:Set) (x:A) : x.val = x := by
+  -- ⊢ ↑x = ↑x
+  have h : x.val = ↑x := by rfl
+  exact h
 
 lemma SetTheory.Set.coe_inj (A:Set) (x y:A) : x.val = y.val ↔ x = y := Subtype.coe_inj
 
@@ -718,38 +776,62 @@ def SetTheory.Set.subtype_mk (A:Set) {x:Object} (hx:x ∈ A) : A := ⟨ x, hx �
 lemma SetTheory.Set.subtype_mk_coe {A:Set} {x:Object} (hx:x ∈ A) : A.subtype_mk hx = x := by rfl
 
 
+
+/-- Axiom 3.6 (axiom of specification) -/
 abbrev SetTheory.Set.specify (A:Set) (P: A → Prop) : Set := SetTheory.specify A P
 
-/-- Axiom 3.6 (axiom of specification) -/
-theorem SetTheory.Set.specification_axiom {A : Set} {P : A → Prop} {x : Object}
+theorem SetTheory.Set.mem_of_mem_specify {A : Set} {P : A → Prop} {x : Object}
   (h: x ∈ A.specify P) : x ∈ A
 := by
-  -- These are equivalent by definition of ⊆, just different ways of saying the same thing:
-  have hxA₁ : A.specify P ⊆ A             := (SetTheory.specification_axiom A P).left
-  have hxA₂ : ∀x, x ∈ A.specify P → x ∈ A := (SetTheory.specification_axiom A P).left
+  have hxA : ∀x, x ∈ A.specify P → x ∈ A := (SetTheory.specification_axiom A P).left
+  exact hxA x h
+
+theorem SetTheory.Set.prop_of_mem_specify {A : Set} {P : A → Prop}
+  {x : Object}
+  (h : x ∈ A.specify P) : P ⟨x, (mem_of_mem_specify h)⟩
+:= by
+  have hxA : x ∈ A := mem_of_mem_specify h
+  have hxP : P ⟨x, hxA⟩ := ((SetTheory.specification_axiom A P).right ⟨x, hxA⟩).mp h
+  exact hxP
+
+theorem SetTheory.Set.mem_specify_of_prop {A : Set} {P : A → Prop} {x : Object}
+  (hxA : x ∈ A)
+  (hPx : P ⟨x, hxA⟩) : x ∈ A.specify P
+:= by
+  exact ((SetTheory.specification_axiom A P).right ⟨x, hxA⟩).mpr hPx
+
+theorem SetTheory.Set.specification_axiom {A : Set} {P : A → Prop} {x : Object}
+  (h : x ∈ A.specify P) : x ∈ A
+:= by
+  -- These are just different ways of saying the same thing
+  have hxA₁ : A.specify P ⊆ A               := (SetTheory.specification_axiom A P).left
+  have hxA₂ : ∀ x, ↑x ∈ A.specify P → x ∈ A := (SetTheory.specification_axiom A P).left
   exact hxA₂ x h
 
-/-- Axiom 3.6 (axiom of specification) -/
+
 theorem SetTheory.Set.specification_axiom' {A : Set}
   (P : A → Prop) (x : A) : x.val ∈ A.specify P ↔ P x
 := by
   have hxP : ∀ (x : A), x.val ∈ A.specify P ↔ P x := (SetTheory.specification_axiom A P).right
   exact hxP x
 
-/-- Axiom 3.6 (axiom of specification) -/
 @[simp]
 theorem SetTheory.Set.specification_axiom'' {A : Set}
   (P : A → Prop) (x : Object) : x ∈ A.specify P ↔ ∃ (h : x ∈ A), P ⟨x, h⟩
 := by
   constructor
-  . intro (h : x ∈ A.specify P)
-    use specification_axiom h
-    simp [← specification_axiom' P, h]
-  . intro ⟨ h, hP ⟩
-    simpa [← specification_axiom' P] using hP
+  · intro (hxAP : x ∈ A.specify P)
+    have hxA : x ∈ A      := mem_of_mem_specify hxAP
+    have hPx : P ⟨x, hxA⟩ := prop_of_mem_specify hxAP
+    exact ⟨hxA, hPx⟩
+  · intro ⟨(hxA : x ∈ A), (hPx : P ⟨x, hxA⟩)⟩
+    have hxAP : x ∈ A.specify P := mem_specify_of_prop hxA hPx
+    exact hxAP
+
 
 theorem SetTheory.Set.specify_subset {A : Set} (P : A → Prop) : A.specify P ⊆ A := by
-  exact (SetTheory.specification_axiom A P).left
+  exact fun x => mem_of_mem_specify
+
 
 theorem SetTheory.Set.specify_congr
   {A A' : Set}
@@ -759,23 +841,23 @@ theorem SetTheory.Set.specify_congr
   (hPP' : (x : Object) → (h : x ∈ A) → (h' : x ∈ A') → P ⟨x, h⟩ ↔ P' ⟨x, h'⟩) :
   A.specify P = A'.specify P'
 := by
-  apply SetTheory.extensionality
-  intro x
+  ext x
   constructor
   . intro (hxAP  : x ∈ A.specify P)  -- ⊢ x ∈ A'.specify P'
-    have hxA     : x ∈ A             := specification_axiom hxAP
+    have hxA     : x ∈ A             := mem_of_mem_specify hxAP
     have hxA'    : x ∈ A'            := hAA' ▸ hxA
-    have hxP     : P  ⟨x, hxA⟩       := (specification_axiom' P ⟨x, hxA⟩).mp hxAP
+    have hxP     : P  ⟨x, hxA⟩       := prop_of_mem_specify hxAP
     have hxP'    : P' ⟨x, hxA'⟩      := (hPP' x hxA hxA').mp hxP
-    have hxAP'   : x ∈ A'.specify P' := (specification_axiom'' P' x).mpr ⟨hxA', hxP'⟩
+    have hxAP'   : x ∈ A'.specify P' := mem_specify_of_prop hxA' hxP'
     exact hxAP'
   . intro (hxAP' : x ∈ A'.specify P') -- ⊢ x ∈ A.specify P
-    have hxA'    : x ∈ A'             := specification_axiom hxAP'
-    have hxA     : x ∈ A              := hAA' ▸ hxA'
-    have hxP'    : P' ⟨x, hxA'⟩       := (specification_axiom' P' ⟨x, hxA'⟩).mp hxAP'
-    have hxP     : P  ⟨x, hxA⟩        := (hPP' x hxA hxA').mpr hxP'
-    have hxAP    : x ∈ A.specify P    := (specification_axiom'' P x).mpr ⟨hxA, hxP⟩
+    have hxA'    : x ∈ A'            := mem_of_mem_specify hxAP'
+    have hxA     : x ∈ A             := hAA' ▸ hxA'
+    have hxP'    : P' ⟨x, hxA'⟩      := prop_of_mem_specify hxAP'
+    have hxP     : P  ⟨x, hxA⟩       := (hPP' x hxA hxA').mpr hxP'
+    have hxAP    : x ∈ A.specify P   := mem_specify_of_prop hxA hxP
     exact hxAP
+
 
 instance SetTheory.Set.instIntersection : Inter Set where
   inter X Y := X.specify (fun x ↦ x.val ∈ Y)
@@ -785,11 +867,31 @@ example (X Y: Set) : X ∩ Y = X.specify (fun x ↦ x.val ∈ Y) := rfl
 
 /-- Definition 3.1.22 (Intersections) -/
 @[simp]
-theorem SetTheory.Set.mem_inter (x:Object) (X Y:Set) : x ∈ (X ∩ Y) ↔ (x ∈ X ∧ x ∈ Y) := by
+theorem SetTheory.Set.mem_inter (x : Object) (X Y : Set) : x ∈ (X ∩ Y) ↔ (x ∈ X ∧ x ∈ Y) := by
   constructor
-  . intro h; have h' := specification_axiom h; simp [h']
-    exact (specification_axiom' _ ⟨ x, h' ⟩).mp h
-  intro ⟨ hX, hY ⟩; exact (specification_axiom' (fun x ↦ x.val ∈ Y) ⟨ x,hX⟩).mpr hY
+  · intro (hxXY : x ∈ X ∩ Y)
+    have hxX : x ∈ X := mem_of_mem_specify hxXY
+    have hxY : x ∈ Y := prop_of_mem_specify hxXY
+    exact ⟨hxX, hxY⟩
+  · intro ⟨hxX, hxY⟩
+    exact mem_specify_of_prop hxX hxY
+
+lemma SetTheory.Set.mem_inter_left {x : Object} {X Y : Set}
+  (h : x ∈ X ∩ Y): x ∈ X
+:= by
+  exact ((mem_inter x X Y).mp h).left
+
+lemma SetTheory.Set.mem_inter_right {x : Object} {X Y : Set}
+  (h : x ∈ X ∩ Y): x ∈ Y
+:= by
+  exact ((mem_inter x X Y).mp h).right
+
+lemma SetTheory.Set.mem_inter_of {x : Object} {X Y : Set}
+  (hxX : x ∈ X)
+  (hxY : x ∈ Y) : x ∈ X ∩ Y
+:= by
+  exact (mem_inter x X Y).mpr ⟨hxX, hxY⟩
+
 
 instance SetTheory.Set.instSDiff : SDiff Set where
   sdiff X Y := X.specify (fun x ↦ x.val ∉ Y)
@@ -799,52 +901,159 @@ example (X Y: Set) : X \ Y = X.specify (fun x ↦ x.val ∉ Y) := rfl
 
 /-- Definition 3.1.26 (Difference sets) -/
 @[simp]
-theorem SetTheory.Set.mem_sdiff (x:Object) (X Y:Set) : x ∈ (X \ Y) ↔ (x ∈ X ∧ x ∉ Y) := by
+theorem SetTheory.Set.mem_sdiff (x : Object) (X Y : Set) : x ∈ (X \ Y) ↔ (x ∈ X ∧ x ∉ Y) := by
   constructor
-  . intro h; have h' := specification_axiom h; simp [h']
-    exact (specification_axiom' _ ⟨ x, h' ⟩ ).mp h
-  intro ⟨ hX, hY ⟩; exact (specification_axiom' (fun x ↦ x.val ∉ Y) ⟨ x, hX⟩ ).mpr hY
+  · intro (hxXY : x ∈ X \ Y)
+    have hxX : x ∈ X := mem_of_mem_specify hxXY
+    have hxY : x ∉ Y := prop_of_mem_specify hxXY
+    exact ⟨hxX, hxY⟩
+  · intro ⟨hxX, hxY⟩
+    exact mem_specify_of_prop hxX hxY
+
+lemma SetTheory.Set.mem_sdiff_left {x : Object} {X Y : Set} (h : x ∈ X \ Y) : x ∈ X :=
+  ((mem_sdiff x X Y).mp h).left
+
+lemma SetTheory.Set.mem_sdiff_right {x : Object} {X Y : Set} (h : x ∈ X \ Y) : x ∉ Y :=
+  ((mem_sdiff x X Y).mp h).right
+
 
 /-- Proposition 3.1.27(d) / Exercise 3.1.6 -/
-theorem SetTheory.Set.inter_comm (A B:Set) : A ∩ B = B ∩ A := by sorry
+theorem SetTheory.Set.inter_comm (A B : Set) : A ∩ B = B ∩ A := by
+  ext x
+  constructor
+  · intro (h : x ∈ A ∩ B)
+    have hxA : x ∈ A := mem_of_mem_specify h
+    have hxB : x ∈ B := prop_of_mem_specify h
+    exact mem_specify_of_prop hxB hxA
+  · intro (h : x ∈ B ∩ A)
+    have hxB : x ∈ B := mem_of_mem_specify h
+    have hxA : x ∈ A := prop_of_mem_specify h
+    exact mem_specify_of_prop hxA hxB
 
 /-- Proposition 3.1.27(b) -/
-theorem SetTheory.Set.subset_union {A X: Set} (hAX: A ⊆ X) : A ∪ X = X := by sorry
+theorem SetTheory.Set.subset_union {A X : Set} (hAX: A ⊆ X) : A ∪ X = X := by
+  ext x
+  constructor
+  · intro (h : x ∈ A ∪ X)
+    rcases (mem_union_cases h) with (hxA : x ∈ A) | (hxX : x ∈ X)
+    · have hxAX : x ∈ A → x ∈ X := hAX x
+      exact hxAX hxA
+    · exact hxX
+  · intro (h : x ∈ X)
+    exact mem_union_right h
 
 /-- Proposition 3.1.27(b) -/
-theorem SetTheory.Set.union_subset {A X: Set} (hAX: A ⊆ X) : X ∪ A = X := by sorry
+theorem SetTheory.Set.union_subset {A X : Set} (hAX : A ⊆ X) : X ∪ A = X := by
+  rw [union_comm]
+  exact subset_union hAX
 
 /-- Proposition 3.1.27(c) -/
 @[simp]
-theorem SetTheory.Set.inter_self (A:Set) : A ∩ A = A := by
-  sorry
+theorem SetTheory.Set.inter_self (A : Set) : A ∩ A = A := by
+  ext x
+  constructor
+  · intro (h : x ∈ A ∩ A)
+    exact mem_of_mem_specify h
+  · intro (h : x ∈ A)
+    exact mem_specify_of_prop h h
 
 /-- Proposition 3.1.27(e) -/
-theorem SetTheory.Set.inter_assoc (A B C:Set) : (A ∩ B) ∩ C = A ∩ (B ∩ C) := by sorry
+theorem SetTheory.Set.inter_assoc (A B C : Set) : (A ∩ B) ∩ C = A ∩ (B ∩ C) := by
+  ext x
+  simp [mem_inter]
+  tauto
 
 /-- Proposition 3.1.27(f) -/
-theorem  SetTheory.Set.inter_union_distrib_left (A B C:Set) :
-    A ∩ (B ∪ C) = (A ∩ B) ∪ (A ∩ C) := by
-  sorry
+theorem  SetTheory.Set.inter_union_distrib_left (A B C : Set) :
+  A ∩ (B ∪ C) = (A ∩ B) ∪ (A ∩ C)
+:= by
+  ext x
+  simp only [mem_inter, mem_union]
+  tauto
 
 /-- Proposition 3.1.27(f) -/
 theorem  SetTheory.Set.union_inter_distrib_left (A B C:Set) :
-    A ∪ (B ∩ C) = (A ∪ B) ∩ (A ∪ C) := by
-  sorry
+    A ∪ (B ∩ C) = (A ∪ B) ∩ (A ∪ C)
+:= by
+  ext x
+  simp only [mem_union, mem_inter]
+  tauto
 
 /-- Proposition 3.1.27(f) -/
-theorem SetTheory.Set.union_compl {A X:Set} (hAX: A ⊆ X) : A ∪ (X \ A) = X := by sorry
+theorem SetTheory.Set.union_compl {A X : Set}
+  (hAX : A ⊆ X) : A ∪ (X \ A) = X
+:= by
+  ext x
+  rw [mem_union, mem_sdiff]
+  constructor
+  · intro (h₁ : x ∈ A ∨ (x ∈ X ∧ x ∉ A))
+    have h₂ : x ∈ A → x ∈ X           := hAX x
+    have h₃ : x ∈ X ∨ (x ∈ X ∧ x ∉ A) := Or.imp_left h₂ h₁
+    have h₄ : x ∈ X                   := by tauto
+    exact h₄
+  · intro (h₁ : x ∈ X)
+    have h₂ : x ∈ A ∨ (x ∈ X ∧ x ∉ A) := by tauto
+    exact h₂
+
+theorem SetTheory.Set.union_compl' {A X : Set}
+  (hAX : A ⊆ X) : A ∪ (X \ A) = X
+:= by
+  ext x
+  rw [mem_union, mem_sdiff]
+  tauto
 
 /-- Proposition 3.1.27(f) -/
-theorem SetTheory.Set.inter_compl {A X:Set} (hAX: A ⊆ X) : A ∩ (X \ A) = ∅ := by sorry
+theorem SetTheory.Set.inter_compl {A X : Set} : A ∩ (X \ A) = ∅
+:= by
+  ext x
+  rw [mem_inter, mem_sdiff]
+  constructor
+  · intro ⟨(hA : x ∈ A), (hX : x ∈ X), (hnA : x ∉ A)⟩
+    exact (hnA hA).elim
+  · intro (h : x ∈ ∅)
+    exact ((not_mem_empty x) h).elim
 
 /-- Proposition 3.1.27(g) -/
-theorem SetTheory.Set.compl_union {A B X:Set} (hAX: A ⊆ X) (hBX: B ⊆ X) :
-    X \ (A ∪ B) = (X \ A) ∩ (X \ B) := by sorry
+theorem SetTheory.Set.compl_union {A B X : Set}
+  (_hAX : A ⊆ X)
+  (_hBX : B ⊆ X) : X \ (A ∪ B) = (X \ A) ∩ (X \ B)
+:= by
+  ext x
+  calc  x ∈ X \ (A ∪ B)
+    _ ↔ x ∈ X ∧ ¬(x ∈ A ∨ x ∈ B)           := by rw [mem_sdiff, mem_union]
+    _ ↔ x ∈ X ∧ x ∉ A ∧ x ∉ B              := by rw [not_or]
+    _ ↔ (x ∈ X ∧ x ∉ A) ∧ (x ∈ X ∧ x ∉ B)  := by rw [and_and_left]
+    _ ↔ (x ∈ X \ A) ∧ (x ∈ X \ B)          := by rw [← mem_sdiff, ← mem_sdiff]
+    _ ↔ x ∈ (X \ A) ∩ (X \ B)              := by rw [← mem_inter]
 
 /-- Proposition 3.1.27(g) -/
-theorem SetTheory.Set.compl_inter {A B X:Set} (hAX: A ⊆ X) (hBX: B ⊆ X) :
-    X \ (A ∩ B) = (X \ A) ∪ (X \ B) := by sorry
+theorem SetTheory.Set.compl_inter {A B X : Set}
+  (_hAX : A ⊆ X)
+  (_hBX : B ⊆ X) : X \ (A ∩ B) = (X \ A) ∪ (X \ B)
+:= by
+  ext x
+  calc  x ∈ X \ (A ∩ B)
+    _ ↔ x ∈ X ∧ ¬(x ∈ A ∧ x ∈ B)          := by rw [mem_sdiff, mem_inter]
+    _ ↔ x ∈ X ∧ (x ∉ A ∨ x ∉ B)           := by rw [not_and_or]
+    _ ↔ (x ∈ X ∧ x ∉ A) ∨ (x ∈ X ∧ x ∉ B) := by rw [and_or_left]
+    _ ↔ x ∈ (X \ A) ∨ x ∈ (X \ B)         := by rw [← mem_sdiff, ← mem_sdiff]
+    _ ↔ x ∈ (X \ A) ∪ (X \ B)             := by rw [← mem_union]
+
+-- In both cases, we can drop the assumptions:
+
+theorem SetTheory.Set.compl_union' {A B X : Set} :
+   X \ (A ∪ B) = (X \ A) ∩ (X \ B)
+:= by
+  ext x
+  simp only [mem_sdiff, mem_union, mem_inter]
+  tauto
+
+theorem SetTheory.Set.compl_inter' {A B X : Set} :
+  X \ (A ∩ B) = (X \ A) ∪ (X \ B)
+:= by
+  ext x
+  simp only [mem_union, mem_sdiff, mem_inter]
+  tauto
 
 /-- Not from textbook: sets form a distributive lattice. -/
 instance SetTheory.Set.instDistribLattice : DistribLattice Set where
@@ -854,15 +1063,23 @@ instance SetTheory.Set.instDistribLattice : DistribLattice Set where
   le_antisymm := subset_antisymm
   inf := (· ∩ ·)
   sup := (· ∪ ·)
-  le_sup_left := by sorry
-  le_sup_right := by sorry
-  sup_le := by sorry
-  inf_le_left := by sorry
-  inf_le_right := by sorry
-  le_inf := by sorry
+
+  le_sup_left := fun A B x hxA => mem_union_left hxA
+  le_sup_right := fun A B x hxB => mem_union_right hxB
+
+  sup_le := fun A B C hAC hBC x hxAB => by
+    cases mem_union_cases hxAB with
+    | inl hxA => exact hAC x hxA
+    | inr hxB => exact hBC x hxB
+
+  inf_le_left := fun A B x hxAB => mem_inter_left hxAB
+  inf_le_right := fun A B x hxAB => mem_inter_right hxAB
+  le_inf := fun A B C hAB hAC x hxA => mem_inter_of (hAB x hxA) (hAC x hxA)
+
   le_sup_inf := by
-    intro X Y Z; change (X ∪ Y) ∩ (X ∪ Z) ⊆ X ∪ (Y ∩ Z)
-    rw [←union_inter_distrib_left]
+    intro X Y Z
+    change (X ∪ Y) ∩ (X ∪ Z) ⊆ X ∪ (Y ∩ Z)
+    rw [← union_inter_distrib_left]
 
 /-- Sets have a minimal element.  -/
 instance SetTheory.Set.instOrderBot : OrderBot Set where
@@ -884,9 +1101,14 @@ abbrev SetTheory.Set.replace (A:Set) {P: A → Object → Prop}
 
 /-- Axiom 3.7 (Axiom of replacement) -/
 @[simp]
-theorem SetTheory.Set.replacement_axiom {A:Set} {P: A → Object → Prop}
-  (hP: ∀ x y y', P x y ∧ P x y' → y = y') (y:Object) :
-    y ∈ A.replace hP ↔ ∃ x, P x y := SetTheory.replacement_axiom A P hP y
+theorem SetTheory.Set.replacement_axiom
+  {A : Set}
+  {P : A → Object → Prop}
+  (hP : ∀ x y y', P x y ∧ P x y' → y = y')
+  (y : Object)
+  : y ∈ A.replace hP ↔ ∃ x, P x y
+:= by
+  exact SetTheory.replacement_axiom A P hP y
 
 abbrev Nat := SetTheory.nat
 
@@ -1014,14 +1236,33 @@ example : ({3, 5}:Set) ⊆ {1, 3, 5} := by
 
 /-- Example 3.1.17 (simplified). -/
 example : ({3, 5}:Set).specify (fun x ↦ x.val ≠ 3) = ({5}:Set) := by
-  ext
-  simp only [mem_singleton, specification_axiom'']
+  ext x
+  simp only [mem_singleton] -- x ∈ {5} → x = 5
   constructor
-  · rintro ⟨h1, h2⟩; simp only [mem_pair] at h1; tauto
-  rintro ⟨rfl⟩; norm_num
+  · intro h₀
+    have h₁ : x ∈ ({3, 5} : Set) := mem_of_mem_specify h₀
+    have h₂ : ↑x ≠ 3             := prop_of_mem_specify h₀
+    rcases (mem_pair x 3 5).mp h₁ with (hx3 : x = 3) | (hx5 : x = 5)
+    · exact (h₂ hx3).elim
+    · exact hx5
+  · intro (hx5 : x = 5)
+    have h₁ : x ∈ ({3, 5} : Set) := mem_pair_right x 3 5 hx5
+    have h₂ : x ≠ 3 := by rw [hx5]; norm_num
+    have h₃ : x ∈ ({3, 5}:Set).specify (fun x ↦ x.val ≠ 3) := mem_specify_of_prop h₁ h₂
+    exact h₃
+
+example : ({3, 5}:Set).specify (fun x ↦ x.val ≠ 3) = ({5}:Set) := by
+  ext x
+  simp only [mem_singleton]
+  constructor
+  · intro h₁
+    simp only [ne_eq, specification_axiom'', mem_pair, exists_prop] at h₁
+    tauto
+  · rintro rfl
+    norm_num
 
 /-- Example 3.1.24 -/
-example : ({1, 2, 4}:Set) ∩ {2,3,4} = {2, 4} := by
+example : ({1, 2, 4}:Set) ∩ {2, 3, 4} = {2, 4} := by
   ext x
   -- Instead of unfolding repetitive branches by hand like earlier,
   -- you can use the `aesop` tactic which does this automatically.
@@ -1030,115 +1271,410 @@ example : ({1, 2, 4}:Set) ∩ {2,3,4} = {2, 4} := by
 /-- Example 3.1.24 -/
 
 example : ({1, 2}:Set) ∩ {3,4} = ∅ := by
-  rw [eq_empty_iff_forall_notMem]
+  rw [eq_empty_iff_forall_not_mem]
   aesop
 
 example : ¬ Disjoint ({1, 2, 3}:Set) {2,3,4} := by
   rw [disjoint_iff]
   intro h
   change {1, 2, 3} ∩ {2, 3, 4} = ∅ at h
-  rw [eq_empty_iff_forall_notMem] at h
+  rw [eq_empty_iff_forall_not_mem] at h
   aesop
 
-example : Disjoint (∅:Set) ∅ := by sorry
+example : Disjoint (∅:Set) ∅ := by
+  rw [disjoint_iff]
+  ext x
+  constructor
+  · intro h
+    exact (not_mem_empty' (mem_inter_left h)).elim
+  · intro h
+    exact (not_mem_empty' h).elim
+
 
 /-- Definition 3.1.26 example -/
 
 example : ({1, 2, 3, 4}:Set) \ {2,4,6} = {1, 3} := by
-  apply ext; aesop
+  ext x
+  aesop
 
 /-- Example 3.1.30 -/
-example : ({3,5,9}:Set).replace (P := fun x y ↦ ∃ (n:ℕ), x.val = n ∧ y = (n+1:ℕ)) (by aesop)
-  = {4,6,10} := by sorry
+example : ({3, 5, 9}:Set).replace (P := fun x y ↦ ∃ (n:ℕ), x.val = n ∧ y = (n+1:ℕ)) (by aesop)
+  = {4,6,10} := by
+  ext x
+  simp only [replacement_axiom]
+  constructor
+  · intro ⟨y, ⟨z, h₁, h₂⟩⟩
+    aesop
+  · intro h₁
+    aesop
 
 /-- Example 3.1.31 -/
 example : ({3,5,9}:Set).replace (P := fun _ y ↦ y=1) (by aesop) = {1} := by
   ext; simp only [replacement_axiom]; aesop
 
 /-- Exercise 3.1.5.  One can use the `tfae_have` and `tfae_finish` tactics here. -/
-theorem SetTheory.Set.subset_tfae (A B:Set) : [A ⊆ B, A ∪ B = B, A ∩ B = A].TFAE := by sorry
+theorem SetTheory.Set.subset_tfae (A B:Set) : [A ⊆ B, A ∪ B = B, A ∩ B = A].TFAE := by
+  tfae_have 1 → 2 := by intro h; ext x; simp [mem_union]; exact h x
+  tfae_have 1 → 3 := by intro h; ext x; simp [mem_inter]; exact h x
+  tfae_have 2 → 1 := by intro h x; rw [h.symm]; simp [mem_union]; tauto
+  tfae_have 3 → 1 := by intro h x; rw [h.symm]; simp [mem_inter]
+  tfae_have 2 → 3 := by intro h; ext x; rw [h.symm]; simp [mem_inter]; tauto
+  tfae_finish
 
 /-- Exercise 3.1.7 -/
-theorem SetTheory.Set.inter_subset_left (A B:Set) : A ∩ B ⊆ A := by
-  sorry
+theorem SetTheory.Set.inter_subset_left (A B:Set) : A ∩ B ⊆ A :=
+  fun _ hxAB => mem_inter_left hxAB
 
 /-- Exercise 3.1.7 -/
-theorem SetTheory.Set.inter_subset_right (A B:Set) : A ∩ B ⊆ B := by
-  sorry
-
-/-- Exercise 3.1.7 -/
-@[simp]
-theorem SetTheory.Set.subset_inter_iff (A B C:Set) : C ⊆ A ∩ B ↔ C ⊆ A ∧ C ⊆ B := by
-  sorry
-
-/-- Exercise 3.1.7 -/
-theorem SetTheory.Set.subset_union_left (A B:Set) : A ⊆ A ∪ B := by
-  sorry
-
-/-- Exercise 3.1.7 -/
-theorem SetTheory.Set.subset_union_right (A B:Set) : B ⊆ A ∪ B := by
-  sorry
+theorem SetTheory.Set.inter_subset_right (A B:Set) : A ∩ B ⊆ B :=
+  fun _ hxAB => mem_inter_right hxAB
 
 /-- Exercise 3.1.7 -/
 @[simp]
-theorem SetTheory.Set.union_subset_iff (A B C:Set) : A ∪ B ⊆ C ↔ A ⊆ C ∧ B ⊆ C := by
-  sorry
+theorem SetTheory.Set.subset_inter_iff (A B C:Set) : C ⊆ A ∩ B ↔ C ⊆ A ∧ C ⊆ B := ⟨
+  fun hCAB => ⟨
+    fun x hxC => mem_inter_left (hCAB x hxC),
+    fun x hxC => mem_inter_right (hCAB x hxC)
+  ⟩,
+  fun ⟨hCA, hCB⟩ x hxC => mem_inter_of (hCA x hxC) (hCB x hxC)
+⟩
+
+/-- Exercise 3.1.7 -/
+theorem SetTheory.Set.subset_union_left (A B:Set) : A ⊆ A ∪ B :=
+  fun _ hxA => mem_union_left hxA
+
+/-- Exercise 3.1.7 -/
+theorem SetTheory.Set.subset_union_right (A B:Set) : B ⊆ A ∪ B :=
+  fun _ hxB => mem_union_right hxB
+
+/-- Exercise 3.1.7 -/
+@[simp]
+theorem SetTheory.Set.union_subset_iff (A B C:Set) : A ∪ B ⊆ C ↔ A ⊆ C ∧ B ⊆ C := ⟨
+  fun hABC => ⟨
+    fun x hxA => hABC x (mem_union_left hxA),
+    fun x hxB => hABC x (mem_union_right hxB)
+  ⟩,
+  fun ⟨hAC, hBC⟩ x hxAB => Or.elim (mem_union_cases hxAB) (hAC x) (hBC x)
+⟩
 
 /-- Exercise 3.1.8 -/
 @[simp]
-theorem SetTheory.Set.inter_union_cancel (A B:Set) : A ∩ (A ∪ B) = A := by sorry
+theorem SetTheory.Set.inter_union_cancel (A B:Set) : A ∩ (A ∪ B) = A := by
+  ext x
+  rw [mem_inter, mem_union]
+  tauto
 
 /-- Exercise 3.1.8 -/
 @[simp]
-theorem SetTheory.Set.union_inter_cancel (A B:Set) : A ∪ (A ∩ B) = A := by sorry
+theorem SetTheory.Set.union_inter_cancel (A B:Set) : A ∪ (A ∩ B) = A := by
+  ext x
+  rw [mem_union, mem_inter]
+  tauto
 
 /-- Exercise 3.1.9 -/
-theorem SetTheory.Set.partition_left {A B X:Set} (h_union: A ∪ B = X) (h_inter: A ∩ B = ∅) :
-    A = X \ B := by sorry
+theorem SetTheory.Set.partition_left {A B X:Set}
+  (h_union: A ∪ B = X)
+  (h_inter: A ∩ B = ∅) : A = X \ B
+:= by
+  ext x
+  rw [mem_sdiff]
+  constructor
+  · intro hxA
+    have hxX : x ∈ X := h_union.symm ▸ (mem_union_left hxA)
+    have hxB : x ∉ B := fun hxB => (not_mem_empty x) (h_inter ▸ (mem_inter_of hxA hxB))
+    exact ⟨hxX, hxB⟩
+  · intro ⟨hxX, hxB⟩
+    have hxAB : x ∈ A ∨ x ∈ B := mem_union_cases (h_union ▸ hxX)
+    have hxA  : x ∈ A         := by tauto
+    exact hxA
 
 /-- Exercise 3.1.9 -/
-theorem SetTheory.Set.partition_right {A B X:Set} (h_union: A ∪ B = X) (h_inter: A ∩ B = ∅) :
-    B = X \ A := by
-  sorry
+theorem SetTheory.Set.partition_right {A B X:Set}
+  (h_union: A ∪ B = X)
+  (h_inter: A ∩ B = ∅) : B = X \ A
+:= by
+  have h_union' : B ∪ A = X := by simpa only [union_comm] using h_union
+  have h_inter' : B ∩ A = ∅ := by simpa only [inter_comm] using h_inter
+  exact partition_left h_union' h_inter'
+
+lemma SetTheory.Set.singleton_subset_of_mem {x : Object} {A : Set}
+  (hxA : x ∈ A) : {x} ⊆ A
+:= by
+  intro y hy
+  rw [mem_singleton] at hy
+  exact hy ▸ hxA
+
+lemma SetTheory.Set.mem_of_singleton_subset {x : Object} {A : Set}
+  (hxA : {x} ⊆ A) : x ∈ A
+:= by
+  exact hxA x ((mem_singleton x x).mpr rfl)
+
+lemma SetTheory.Set.disjoint_iff_inter_eq_empty {A B : Set} : Disjoint A B ↔ A ∩ B = ∅ := by
+  constructor
+  · intro (h₁ : Disjoint A B)
+    have h_disjoint : ∀X, X ⊆ A → X ⊆ B → X ⊆ ∅ := by simpa only [Disjoint] using h₁
+    ext x
+    constructor
+    · intro (h_inter : x ∈ A ∩ B)
+      have hxA : {x} ⊆ A := singleton_subset_of_mem (mem_inter_left h_inter)
+      have hxB : {x} ⊆ B := singleton_subset_of_mem (mem_inter_right h_inter)
+      have hx0 : x ∈ ∅ := mem_of_singleton_subset (h_disjoint {x} hxA hxB)
+      exact hx0
+    · intro hx0
+      exact (not_mem_empty' hx0).elim
+  · intro (h_inter_empty : A ∩ B = ∅) X (hXA : X ⊆ A) (hXB : X ⊆ B) x (hxX : x ∈ X)
+    have hxAB : x ∈ A ∩ B := mem_inter_of (hXA x hxX) (hXB x hxX)
+    have hx0  : x ∈ ∅ := h_inter_empty ▸ hxAB
+    exact hx0
 
 /--
   Exercise 3.1.10.
   You may find `Function.onFun_apply` and the `fin_cases` tactic useful.
 -/
-theorem SetTheory.Set.pairwise_disjoint (A B:Set) :
-    Pairwise (Function.onFun Disjoint ![A \ B, A ∩ B, B \ A]) := by sorry
+theorem SetTheory.Set.pairwise_disjoint (A B : Set) :
+  Pairwise (Function.onFun Disjoint ![A \ B, A ∩ B, B \ A])
+:= by
+  have h₁ : (A \ B) ∩ (A ∩ B) = ∅ := by ext x; simp [mem_inter, mem_sdiff]; tauto
+  have h₂ : (A \ B) ∩ (B \ A) = ∅ := by ext x; simp [mem_inter, mem_sdiff]; tauto
+  have h₃ : (A ∩ B) ∩ (B \ A) = ∅ := by ext x; simp [mem_inter, mem_sdiff]; tauto
+  intro i j hij
+  fin_cases i <;> fin_cases j <;> try contradiction
+  all_goals simp [disjoint_iff_inter_eq_empty]
+  · exact h₁
+  · exact h₂
+  · simpa [inter_comm] using h₁
+  · exact h₃
+  · simpa [inter_comm] using h₂
+  · simpa [inter_comm] using h₃
 
 /-- Exercise 3.1.10 -/
-theorem SetTheory.Set.union_eq_partition (A B:Set) : A ∪ B = (A \ B) ∪ (A ∩ B) ∪ (B \ A) := by
-  sorry
+theorem SetTheory.Set.union_eq_partition (A B : Set) : A ∪ B = (A \ B) ∪ (A ∩ B) ∪ (B \ A) := by
+  ext x
+  simp only [mem_union, mem_sdiff, mem_inter]
+  tauto
 
 /--
   Exercise 3.1.11.
   The challenge is to prove this without using `Set.specify`, `Set.specification_axiom`,
   `Set.specification_axiom'`, or anything built from them (like differences and intersections).
 -/
-theorem SetTheory.Set.specification_from_replacement {A:Set} {P: A → Prop} :
-    ∃ B, B ⊆ A ∧ ∀ x, x.val ∈ B ↔ P x := by sorry
+theorem SetTheory.Set.specification_from_replacement {A : Set} {P : A → Prop} :
+  ∃ B, B ⊆ A ∧ ∀ x, x.val ∈ B ↔ P x
+:= by
+  let P' : (Subtype (mem · A)) → Object → Prop := fun x y => (↑x = y) ∧ P x
+  have hP' : ∀ (x : Subtype (mem · A)) (y y' : Object), P' x y ∧ P' x y' → y = y' := by
+    intro x y y' ⟨⟨(hxy : x = y), _⟩, ⟨(hxy' : x = y'), _⟩⟩
+    exact hxy ▸ hxy'
+  let B := replace A hP'
+  use B
+  have hB : B ⊆ A := by
+    intro x (hxB : x ∈ B)
+    have h₁ : ∃ z, ∃ (hzA : z ∈ A), P' ⟨z, hzA⟩ x := by simpa [B] using hxB
+    have ⟨z, hzA, hP'⟩           := h₁
+    have h₂ : z = x ∧ P ⟨z, hzA⟩ := by simpa only [P'] using hP'
+    have hxA : x ∈ A             := h₂.left ▸ hzA
+    exact hxA
+  apply And.intro hB
+  intro (z : A)
+  have h₁ : ↑z ∈ B ↔ ∃x, P' x z     := replacement_axiom hP' z
+  have h₂ : ↑z ∈ B ↔ (↑z ∈ A) ∧ P z := by simpa [P'] using h₁
+  have h₃ : ↑z ∈ B ↔ P z            := by simpa [z.property] using h₂
+  exact h₃
+
 
 /-- Exercise 3.1.12.-/
-theorem SetTheory.Set.subset_union_subset {A B A' B':Set} (hA'A: A' ⊆ A) (hB'B: B' ⊆ B) :
-    A' ∪ B' ⊆ A ∪ B := by sorry
+theorem SetTheory.Set.subset_union_subset {A B A' B' : Set}
+  (hA'A : A' ⊆ A)
+  (hB'B : B' ⊆ B) : A' ∪ B' ⊆ A ∪ B
+:= by
+  intro x hx
+  rcases (mem_union_cases hx) with hxA' | hxB'
+  · exact mem_union_left (hA'A x hxA')
+  · exact mem_union_right (hB'B x hxB')
 
 /-- Exercise 3.1.12.-/
-theorem SetTheory.Set.subset_inter_subset {A B A' B':Set} (hA'A: A' ⊆ A) (hB'B: B' ⊆ B) :
-    A' ∩ B' ⊆ A ∩ B := by sorry
+theorem SetTheory.Set.subset_inter_subset {A B A' B' : Set}
+  (hA'A : A' ⊆ A)
+  (hB'B : B' ⊆ B) : A' ∩ B' ⊆ A ∩ B
+:= by
+  intro x hx
+  exact mem_inter_of
+    (hA'A x (mem_inter_left hx))
+    (hB'B x (mem_inter_right hx))
+
+lemma SetTheory.Set.sdiff_empty (A : Set) : A \ ∅ = A := by
+  ext x
+  constructor
+  · exact fun hx => mem_of_mem_specify hx
+  · exact fun hx => mem_specify_of_prop hx (not_mem_empty x)
+
+lemma SetTheory.Set.sdiff_self (A : Set) : A \ A = (∅ : Set) := by
+  ext x
+  constructor
+  · intro hx
+    have h₁ := mem_of_mem_specify hx
+    have h₂ := prop_of_mem_specify hx
+    exact (h₂ h₁).elim
+  · intro hx
+    exact (not_mem_empty' hx).elim
 
 /-- Exercise 3.1.12.-/
 theorem SetTheory.Set.subset_diff_subset_counter :
-    ∃ (A B A' B':Set), (A' ⊆ A) ∧ (B' ⊆ B) ∧ ¬ (A' \ B') ⊆ (A \ B) := by sorry
+  ∃ (A B A' B' : Set), (A' ⊆ A) ∧ (B' ⊆ B) ∧ ¬ (A' \ B') ⊆ (A \ B)
+:= by
+  -- Consider any non-empty set X.  Let A = B = A' = X and let B' = ∅
+  -- Then A' \ B' = X \ ∅ = X but A \ B = X \ X = ∅; clearly X ⊆ ∅ is false
+  let X := ({1} : Set)
+  use X; use X; use X; use ∅
+  have h₁ : X ⊆ X     := fun x hx => hx
+  have h₂ : ∅ ⊆ X     := fun x hx => (not_mem_empty' hx).elim
+  have h₃ : X \ ∅ = X := sdiff_empty X
+  have h₄ : X \ X = ∅ := sdiff_self X
+  have h₅ : ¬ X ⊆ ∅   := fun h => not_mem_empty' (h 1 (mem_singleton' 1))
+  simp only [h₁, h₂, h₃, h₄, h₅]
+  tauto
 
 /-
   Final part of Exercise 3.1.12: state and prove a reasonable substitute positive result for the
   above theorem that involves set differences.
 -/
+theorem SetTheory.Set.subset_diff_subset_counter' {A B A' B' : Set}
+  (hA'A : A' ⊆ A)
+  (hB'B : B' ⊆ B) : (A' \ B) ⊆ (A \ B')
+:= by
+  intro x (hxA'B : x ∈ A' \ B)
+  have hxA' : x ∈ A' := mem_of_mem_specify hxA'B
+  have hxB  : x ∉ B  := prop_of_mem_specify hxA'B
+  have hxB' : x ∉ B' := (mt (hB'B x)) hxB
+  have hxA  : x ∈ A  := hA'A x hxA'
+  exact mem_specify_of_prop hxA hxB'
+
+
+lemma SetTheory.Set.exists_distinct_mem_of_nonempty_nonsingleton {A : Set}
+  (x : Object)
+  (h₁ : A ≠ ∅)
+  (h₂ : ∀ a, A ≠ {a}) : ∃y ∈ A, y ≠ x
+:= by
+  contrapose! h₂ -- ∀ y ∈ A, y = x
+  use x
+  ext y
+  constructor
+  · intro (hyA : y ∈ A)
+    have hyx : y = x := h₂ y hyA
+    have hyX : y ∈ {x} := mem_singleton_of_eq hyx
+    exact hyX
+  · intro (hyX : y ∈ ({x} : Set))
+    have ⟨z, (hzA : z ∈ A)⟩ := nonempty_def h₁
+    have hyx : y = x := eq_of_mem_singleton hyX
+    have hzx : z = x := h₂ z hzA
+    have hyA : y ∈ A := hyx ▸ hzx ▸ hzA
+    exact hyA
+
+lemma SetTheory.Set.pair_subset_of_mems {x y : Object} {A : Set}
+  (hxA : x ∈ A)
+  (hyA : y ∈ A) : {x, y} ⊆ A
+:= by
+  intro a ha
+  rcases (mem_pair a x y).mp ha with (hax : a = x) | (hay : a = y)
+  · exact hax ▸ hxA
+  . exact hay ▸ hyA
+
+lemma SetTheory.Set.singleton_ssubset_pair
+  (x y : Object) (hxy : x ≠ y) : {x} ⊂ ({x, y} : Set)
+:= by
+  have h₁ : {x} ⊆ ({x, y} : Set) := fun a => by simp [mem_singleton]; tauto
+  have h₂ : {x} ≠ ({x, y} : Set) := by
+    intro h_eq
+    have hy₁ : y ∈ ({x, y} : Set) := mem_pair_right y x y rfl
+    have hy₂ : y ∈ ({x} : Set)    := h_eq ▸ hy₁
+    have hy₃ : y = x              := eq_of_mem_singleton hy₂
+    exact (hxy hy₃.symm).elim
+  exact ⟨h₁, h₂⟩
+
+lemma SetTheory.Set.singleton_ne_empty (x : Object) :
+  ({x} : Set) ≠ ∅
+:= by
+  by_contra! h₀
+  have h₁ : x ∈ {x} := mem_singleton_of_eq rfl
+  have h₂ : x ∈ ∅   := h₀ ▸ h₁
+  have h₃ : x ∉ ∅   := not_mem_empty x
+  exact (h₃ h₂).elim
+
+lemma SetTheory.Set.subsets_of_singleton {x : Object} {A : Set}
+  (h : A ⊆ {x}) : A = ∅ ∨ A = {x}
+:= by
+  by_cases hA : A = ∅
+  · exact Or.inl hA
+  · have hA' : A = {x} := by
+      ext z
+      constructor
+      · intro (hzA : z ∈ A)
+        exact (h z hzA : z ∈ {x})
+      · intro hzX
+        have ⟨y, (hyA : y ∈ A)⟩ := nonempty_def hA
+        have hyx : y = x := eq_of_mem_singleton (h y hyA)
+        have hzx : z = x := eq_of_mem_singleton hzX
+        have hzA : z ∈ A := hzx ▸ hyx ▸ hyA
+        exact hzA
+    exact Or.inr hA'
+
+lemma SetTheory.Set.ssubset_of_singleton {x : Object} {A : Set}
+  (h : A ⊂ {x}) : A = ∅
+:= by
+  rcases (subsets_of_singleton h.left) with (hA0 : A = ∅) | (hAX : A = {x})
+  · exact hA0
+  · exact (h.right hAX).elim
+
+-- Original version of ssubset_of_singleton, that was shorter, but at the cost
+-- of being much more convoluted in its reasoning
+lemma SetTheory.Set.ssubset_of_singleton' {x : Object} {A : Set}
+  (h : A ⊂ {x}) : A = ∅
+:= by
+  ext y
+  constructor
+  · intro (hyA : y ∈ A)
+    have hyX : y ∈ {x} := h.left y hyA
+    have hyx : y = x   := eq_of_mem_singleton hyX
+    have hxA : x ∈ A   := hyx ▸ hyA
+    have ⟨z, hz⟩       := exists_dist_elem_of_ssubset h
+    have hzx  : z = x  := eq_of_mem_singleton hz.left
+    have hxA' : x ∉ A  := hzx ▸ hz.right
+    exact (hxA' hxA).elim
+  · intro (hy0 : y ∈ ∅)
+    exact (not_mem_empty' hy0).elim
 
 /-- Exercise 3.1.13 -/
-theorem SetTheory.Set.singleton_iff (A:Set) (hA: A ≠ ∅) : (¬∃ B ⊂ A, B ≠ ∅) ↔ ∃ x, A = {x} := by sorry
+theorem SetTheory.Set.singleton_iff
+  (A : Set)
+  (hA : A ≠ ∅) : (¬∃ B ⊂ A, B ≠ ∅) ↔ ∃ x, A = {x}
+:= by
+  constructor
+
+  -- Assume A is a non-empty set whose only proper subset is empty; then for contradiction, assume A
+  -- is not a singleton, so has least two members.  The singleton of either member is a non-empty
+  -- proper subset, but A has no non-empty proper subsets.  Therefore A must be a singleton.
+  · intro h₁
+    push_neg at h₁ -- ∀ B ⊂ A, B = ∅
+    by_contra! h₂ -- ∀ x, A ≠ {x}
+    have ⟨x, (hxA : x ∈ A)⟩ := nonempty_def hA
+    have h₃ : ∃y ∈ A, y ≠ x := exists_distinct_mem_of_nonempty_nonsingleton x hA h₂
+    have ⟨y, hyA, hyx⟩      := h₃
+    have h₄ : {x, y} ⊆ A    := pair_subset_of_mems hxA hyA
+    have h₅ : {x} ⊂ {x, y}  := singleton_ssubset_pair x y hyx.symm
+    have h₆ : {x} ⊂ A       := ssubset_of_ssubset_of_subset h₅ h₄
+    have h₇ : {x} = ∅       := h₁ {x} h₆
+    have h₈ : {x} ≠ ∅       := singleton_ne_empty x
+    exact (h₈ h₇).elim
+
+    -- Assume A is a singleton, and for contradiction that all proper subsets of A are non-empty;
+    -- since the only proper subset of a singleton is the empty set, conclude that no non-empty
+    -- proper subsets of A exist.
+  · intro h₁
+    by_contra! h₂
+    have ⟨x, (hAx : A = {x})⟩ := h₁
+    have ⟨Y, (hYA : Y ⊂ A), (hY0 : Y ≠ ∅)⟩ := h₂
+    have hY0' : Y = ∅ := ssubset_of_singleton (hAx ▸ hYA)
+    exact (hY0 hY0').elim
 
 
 /-
@@ -1149,59 +1685,148 @@ theorem SetTheory.Set.singleton_iff (A:Set) (hA: A ≠ ∅) : (¬∃ B ⊂ A, B 
 instance SetTheory.Set.inst_coe_set : Coe Set (_root_.Set Object) where
   coe X := { x | x ∈ X }
 
+instance SetTheory.Set.inst_coe_set' : Coe (_root_.Set Object) Set where
+  coe X := (univ.specify (fun x => ↑x ∈ X))
+
 -- Now we can convert our `Set` into a Mathlib `_root_.Set`.
 -- Notice that Mathlib sets are parameterized by the element type, in our case `Object`.
-example (X: Set) : _root_.Set Object := X
+example (X : Set) : _root_.Set Object := X
 
 /--
   Injectivity of the coercion. Note however that we do NOT assert that the coercion is surjective
   (and indeed Russell's paradox prevents this)
 -/
 @[simp]
-theorem SetTheory.Set.coe_inj' (X Y:Set) :
-    (X : _root_.Set Object) = (Y : _root_.Set Object) ↔ X = Y := by
+theorem SetTheory.Set.coe_inj' (X Y : Set) :
+  (X : _root_.Set Object) = (Y : _root_.Set Object) ↔ X = Y
+:= by
   constructor
-  . intro h; apply ext; intro x
-    replace h := congr(x ∈ $h); simpa using h
-  rintro rfl; rfl
+  · intro (h₁ : {x | x ∈ X} = {x | x ∈ Y})
+    ext x -- ⊢ x ∈ X ↔ x ∈ Y
+    have h₂ : (x ∈ {x | x ∈ X}) = (x ∈ {x | x ∈ Y}) := congr(x ∈ $h₁)
+    have h₃ : (x ∈ X) = (x ∈ Y) := by simpa only [Set.mem_setOf_eq] using h₂
+    have h₄ : x ∈ X ↔ x ∈ Y     := by simpa only [eq_iff_iff] using h₃
+    exact h₄
+  · rintro (rfl : X = Y)
+    have h₁ : {x | x ∈ X} = {x | x ∈ X} := by rfl
+    exact h₁
 
 /-- Compatibility of the membership operation ∈ -/
-theorem SetTheory.Set.mem_coe (X:Set) (x:Object) : x ∈ (X : _root_.Set Object) ↔ x ∈ X := by
-  simp
+theorem SetTheory.Set.mem_coe (X : Set) (x : Object) : x ∈ (X : _root_.Set Object) ↔ x ∈ X := by
+  simp only [Set.mem_setOf_eq]
 
 /-- Compatibility of the emptyset -/
-theorem SetTheory.Set.coe_empty : ((∅:Set) : _root_.Set Object) = ∅ := by sorry
+theorem SetTheory.Set.coe_empty : ((∅ : Set) : _root_.Set Object) = ∅ := by
+  ext x
+  simp only [Set.mem_setOf_eq]
+  constructor
+  · intro (h : x ∈ (∅ : Set))
+    exact not_mem_empty x h
+  · intro (h : x ∈ ∅)
+    exact ((Set.notMem_empty x) h).elim
 
 /-- Compatibility of subset -/
-theorem SetTheory.Set.coe_subset (X Y:Set) :
-    (X : _root_.Set Object) ⊆ (Y : _root_.Set Object) ↔ X ⊆ Y := by sorry
+theorem SetTheory.Set.coe_subset (X Y : Set) :
+  (X : _root_.Set Object) ⊆ (Y : _root_.Set Object) ↔ X ⊆ Y
+:= by
+  constructor
+  · intro (hXY : {x | x ∈ X} ⊆ {x | x ∈ Y})
+    intro x (hxX : x ∈ X)
+    have hxX' : x ∈ {x | x ∈ X} := Set.mem_setOf_eq.mpr hxX
+    have hxY' : x ∈ {x | x ∈ Y} := Set.mem_of_mem_of_subset hxX' hXY
+    have hxY  : x ∈ Y           := Set.mem_setOf_eq.mp hxY'
+    exact hxY
+  · intro (hXY : X ⊆ Y)
+    simp only [Set.setOf_subset_setOf]
+    exact hXY
 
-theorem SetTheory.Set.coe_ssubset (X Y:Set) :
-    (X : _root_.Set Object) ⊂ (Y : _root_.Set Object) ↔ X ⊂ Y := by sorry
+theorem SetTheory.Set.coe_ssubset (X Y : Set) :
+  (X : _root_.Set Object) ⊂ (Y : _root_.Set Object) ↔ X ⊂ Y
+:= by
+  constructor
+  · intro (hXY₁ : {x | x ∈ X} ⊂ {x | x ∈ Y})
+    have ⟨hXY₂, ⟨x, hxY₁, hxX₁⟩⟩ := Set.ssubset_iff_exists.mp hXY₁
+    have hxY₂ : x ∈ Y := Set.mem_setOf_eq.mpr hxY₁
+    have hxX₂ : x ∉ X := Set.notMem_setOf_iff.mpr hxX₁
+    have hXY₃ : X ⊂ Y := ssubset_of_subset_of_dist_elem hXY₂ ⟨x, hxY₂, hxX₂⟩
+    exact hXY₃
+  · intro (hXY₁ : X ⊂ Y)
+    have hXY₂ : X ⊆ Y := hXY₁.left
+    have hXY₃ : {x | x ∈ X} ⊆ {x | x ∈ Y} := by simpa [Set.mem_setOf_eq] using hXY₂
+    have ⟨x, hxY, hxX⟩ := exists_dist_elem_of_ssubset hXY₁
+    have h := Set.ssubset_iff_exists.mpr ⟨hXY₃, ⟨x, hxY, hxX⟩⟩
+    exact h
 
 /-- Compatibility of singleton -/
-theorem SetTheory.Set.coe_singleton (x: Object) : ({x} : _root_.Set Object) = {x} := by sorry
+theorem SetTheory.Set.coe_singleton (x: Object) : ({x} : _root_.Set Object) = {x} := by
+  rfl
 
 /-- Compatibility of union -/
-theorem SetTheory.Set.coe_union (X Y: Set) :
-    (X ∪ Y : _root_.Set Object) = (X : _root_.Set Object) ∪ (Y : _root_.Set Object) := by sorry
+theorem SetTheory.Set.coe_union (X Y : Set) :
+  (X ∪ Y : _root_.Set Object) = (X : _root_.Set Object) ∪ (Y : _root_.Set Object)
+:= by
+  ext x
+  simp [Set.mem_setOf_eq]
 
 /-- Compatibility of pair -/
-theorem SetTheory.Set.coe_pair (x y: Object) : ({x, y} : _root_.Set Object) = {x, y} := by sorry
+theorem SetTheory.Set.coe_pair (x y : Object) : ({x, y} : _root_.Set Object) = {x, y} := by
+  rfl
 
 /-- Compatibility of subtype -/
-theorem SetTheory.Set.coe_subtype (X: Set) :  (X : _root_.Set Object) = X.toSubtype := by sorry
+theorem SetTheory.Set.coe_subtype (X : Set) :  (X : _root_.Set Object) = X.toSubtype := by
+  rfl
 
 /-- Compatibility of intersection -/
 theorem SetTheory.Set.coe_intersection (X Y: Set) :
-    (X ∩ Y : _root_.Set Object) = (X : _root_.Set Object) ∩ (Y : _root_.Set Object) := by sorry
+  (X ∩ Y : _root_.Set Object) = (X : _root_.Set Object) ∩ (Y : _root_.Set Object)
+:= by
+  ext x
+  simp [Set.mem_setOf_eq]
 
 /-- Compatibility of set difference-/
-theorem SetTheory.Set.coe_diff (X Y: Set) :
-    (X \ Y : _root_.Set Object) = (X : _root_.Set Object) \ (Y : _root_.Set Object) := by sorry
+theorem SetTheory.Set.coe_diff (X Y : Set) :
+  (X \ Y : _root_.Set Object) = (X : _root_.Set Object) \ (Y : _root_.Set Object)
+:= by
+  ext x
+  simp [Set.mem_setOf_eq]
 
 /-- Compatibility of disjointness -/
-theorem SetTheory.Set.coe_Disjoint (X Y: Set) :
-    Disjoint (X : _root_.Set Object) (Y : _root_.Set Object) ↔ Disjoint X Y := by sorry
+theorem SetTheory.Set.coe_Disjoint (X Y : Set) :
+  Disjoint (X : _root_.Set Object) (Y : _root_.Set Object) ↔ Disjoint X Y
+:= by
+  constructor
+  · intro (h₁ : Disjoint {x | x ∈ X} {x | x ∈ Y})
+    simp [Disjoint] at *
+    intro Z (hZX : Z ⊆ X) (hZY : Z ⊆ Y)
+    have h₂ : {x | x ∈ Z} ⊆ {x | x ∈ X} := by simpa only [Set.setOf_subset_setOf] using hZX
+    have h₃ : {x | x ∈ Z} ⊆ {x | x ∈ Y} := by simpa only [Set.setOf_subset_setOf] using hZY
+    have h₄ : {x | x ∈ Z} = ∅           := h₁ h₂ h₃
+    have h₅ : ∀ x, x ∉ {x | x ∈ Z}      := Set.eq_empty_iff_forall_notMem.mp h₄
+    have h₆ : ∀ x, x ∉ Z                := by simpa only [Set.notMem_setOf_iff] using h₅
+    have h₇ : Z = ∅                     := eq_empty_iff_forall_not_mem.mpr h₆
+    exact h₇
+  · intro (h₁ : Disjoint X Y)
+    simp [Disjoint] at *
+    intro Z (hZX₁ : Z ⊆ {x | x ∈ X}) (hZY₁ : Z ⊆ {x | x ∈ Y})
+    let Z' : Set := Z
+    ext x
+    constructor
+    · intro (hxZ : x ∈ Z)
+      have hZX : Z' ⊆ X := by
+        intro y (hyZ' : y ∈ Z')
+        have hyZ : y ∈ univ ∧ y ∈ Z  := by simpa [Z'] using hyZ'
+        have hyX : y ∈ X             := by simpa only [Set.mem_setOf_eq] using (hZX₁ hyZ.right)
+        exact hyX
+      have hZY : Z' ⊆ Y := by
+        intro y (hyZ' : y ∈ Z')
+        have hyZ : y ∈ univ ∧ y ∈ Z  := by simpa [Z'] using hyZ'
+        have hyY : y ∈ Y             := by simpa only [Set.mem_setOf_eq] using (hZY₁ hyZ.right)
+        exact hyY
+      have hxZ' : x ∈ Z'             := by simpa [Z'] using ⟨SetTheory.mem_univ x, hxZ⟩
+      have hZ0  : Z' = ∅             := h₁ hZX hZY
+      have hx0  : x ∈ ∅              := hZ0 ▸ hxZ'
+      exact not_mem_empty' hx0
+    · intro (hx0₁ : x ∈ ∅)
+      exact ((Set.notMem_empty x) hx0₁).elim
 
 end Chapter3
